Finish proof n_hashes_acc

Cook_Levin/IMP-_To_SAS+/IMP-_To_IMP--/IMP_Minus_To_IMP_Minus_Minus_State_Translations_IMP.thy
@@ -4,136 +4,295 @@ theory IMP_Minus_To_IMP_Minus_Minus_State_Translations_IMP
           IMP_Minus.Com
 begin
 
-record n_hashes_state =
-  n_hashes_acc::nat
-  n_hashes_n::nat
+unbundle IMP_Minus_Minus_Com.no_com_syntax
 
-abbreviation "n_hashes_prefix \<equiv> ''n_hashes.''"
-abbreviation "n_hashes_acc_str \<equiv> ''acc''"
-abbreviation "n_hashes_n_str \<equiv> ''n''"
+record n_hashes_acc_state =
+  n_hashes_acc_acc::nat
+  n_hashes_acc_n::nat
+  n_hashes_acc_ret::nat
 
-lemma pound_encode_val: "encode_char (CHR ''#'') = 35" by eval
+abbreviation "n_hashes_acc_prefix \<equiv> ''n_hashes_acc.''"
+abbreviation "n_hashes_acc_acc_str \<equiv> ''acc''"
+abbreviation "n_hashes_acc_n_str \<equiv> ''n''"
+abbreviation "n_hashes_acc_ret_str \<equiv> ''ret''"
 
-definition "n_hashes_state_upd s \<equiv>
+abbreviation "hash_as_nat \<equiv> 35"
+lemma hash_encode_val: "encode_char (CHR ''#'') = hash_as_nat"
+  by (simp add: encode_char_def)
+
+definition "n_hashes_acc_state_upd s \<equiv>
       let
-        cons_h' = 35;
-        cons_t' = n_hashes_acc s;
+        cons_h' = hash_as_nat;
+        cons_t' = n_hashes_acc_acc s;
         cons_ret' = 0;
         cons_state = \<lparr>cons_h = cons_h', cons_t = cons_t', cons_ret = cons_ret'\<rparr>;
         cons_ret_state = cons_imp cons_state;
-        n_hashes_acc' = cons_ret cons_ret_state;
-        n_hashes_n' = n_hashes_n s - 1;
-        ret = \<lparr>n_hashes_acc = n_hashes_acc', n_hashes_n = n_hashes_n'\<rparr>
+        n_hashes_acc_acc' = cons_ret cons_ret_state;
+        n_hashes_acc_n' = n_hashes_acc_n s - 1;
+        ret = \<lparr>n_hashes_acc_acc = n_hashes_acc_acc',
+               n_hashes_acc_n = n_hashes_acc_n',
+               n_hashes_acc_ret = n_hashes_acc_ret s\<rparr>
       in
         ret
 "
 
-function n_hashes_imp:: "n_hashes_state \<Rightarrow> n_hashes_state" where
-  "n_hashes_imp s = 
-  (if n_hashes_n s \<noteq> 0
+definition "n_hashes_acc_imp_compute_loop_condition s \<equiv>
+  (let
+    condition = n_hashes_acc_n s
+   in condition
+  )"
+
+definition "n_hashes_acc_imp_after_loop s \<equiv>
+  (let
+    ret = \<lparr>n_hashes_acc_acc = n_hashes_acc_acc s,
+           n_hashes_acc_n = n_hashes_acc_n s,
+           n_hashes_acc_ret = n_hashes_acc_acc s\<rparr>
+   in ret
+  )"
+
+lemmas n_hashes_acc_imp_subprogram_simps =
+  n_hashes_acc_imp_after_loop_def
+  n_hashes_acc_state_upd_def
+  n_hashes_acc_imp_compute_loop_condition_def
+
+function n_hashes_acc_imp:: "n_hashes_acc_state \<Rightarrow> n_hashes_acc_state" where
+  "n_hashes_acc_imp s =
+  (if n_hashes_acc_imp_compute_loop_condition s \<noteq> 0
    then
-    (let next_iteration = n_hashes_imp (n_hashes_state_upd s)
+    (let next_iteration = n_hashes_acc_imp (n_hashes_acc_state_upd s)
       in next_iteration)
   else
-    (let ret = s in ret)
+    (let ret = n_hashes_acc_imp_after_loop s in ret)
   )"
   by simp+
-termination by (relation "measure (\<lambda>s. n_hashes_n s)") (simp add: n_hashes_state_upd_def)+
+termination by (relation "measure (\<lambda>s. n_hashes_acc_n s)")
+    (simp add: n_hashes_acc_imp_subprogram_simps)+
 
-declare n_hashes_imp.simps [simp del]
+declare n_hashes_acc_imp.simps [simp del]
 
-lemma n_hashes_imp_correct:
-  "n_hashes_acc (n_hashes_imp s)
-    = IMP_Minus_To_IMP_Minus_Minus_State_Translations_nat.n_hashes_acc
-        (n_hashes_acc s) (n_hashes_n s)"
-proof (induction s rule: n_hashes_imp.induct)
-  case (1 s)
-  then show ?case
-    apply(subst n_hashes_imp.simps)
-    by (auto simp: n_hashes_state_upd_def Let_def)
-      (metis Suc_pred cons_imp_correct cons_state.simps(1) cons_state.simps(2)
-        n_hashes_acc.simps(2) pound_encode_val)
-qed 
+lemma n_hashes_acc_imp_correct:
+  "n_hashes_acc_ret (n_hashes_acc_imp s) = n_hashes_acc (n_hashes_acc_acc s) (n_hashes_acc_n s)"
+  apply(induction s rule: n_hashes_acc_imp.induct)
+  apply(subst n_hashes_acc_imp.simps)
+  apply(simp add: n_hashes_acc_imp_subprogram_simps cons_imp_correct hash_encode_val Suc_diff_Suc)
+  by (metis Suc_pred hash_encode_val n_hashes_acc.simps(2))
 
-function n_hashes_imp_time:: "nat \<Rightarrow> n_hashes_state \<Rightarrow> nat" where
-  "n_hashes_imp_time t s =
-  (if n_hashes_n s \<noteq> 0
-   then
-    (let
-        cons_h' = 35;
+definition "n_hashes_acc_state_upd_time t s \<equiv>
+      let
+        cons_h' = hash_as_nat;
         t = t + 2;
-        cons_t' = n_hashes_acc s;
+        cons_t' = n_hashes_acc_acc s;
         t = t + 2;
         cons_ret' = 0;
         t = t + 2;
         cons_state = \<lparr>cons_h = cons_h', cons_t = cons_t', cons_ret = cons_ret'\<rparr>;
         cons_ret_state = cons_imp cons_state;
         t = t + cons_imp_time 0 cons_state;
-        n_hashes_acc' = cons_ret cons_ret_state;
+        n_hashes_acc_acc' = cons_ret cons_ret_state;
         t = t + 2;
-        n_hashes_n' = n_hashes_n s - 1;
+        n_hashes_acc_n' = n_hashes_acc_n s - 1;
         t = t + 2;
-        next_iteration = n_hashes_imp_time t (n_hashes_state_upd s)
+        ret = t
+      in
+        ret
+"
+
+definition "n_hashes_acc_imp_compute_loop_condition_time t s \<equiv>
+  (let
+    condition = n_hashes_acc_n s;
+    t = t + 2;
+    ret = t
+   in ret
+  )"
+
+definition "n_hashes_acc_imp_after_loop_time t s \<equiv>
+  (let
+    t = t + 2;
+    ret = t
+   in ret
+  )"
+
+function n_hashes_acc_imp_time:: "nat \<Rightarrow> n_hashes_acc_state \<Rightarrow> nat" where
+  "n_hashes_acc_imp_time t s =
+  n_hashes_acc_imp_compute_loop_condition_time 0 s +
+  (if n_hashes_acc_imp_compute_loop_condition s \<noteq> 0
+   then
+    (let
+        t = t + 1;
+        next_iteration
+          = n_hashes_acc_imp_time (t + n_hashes_acc_state_upd_time 0 s) (n_hashes_acc_state_upd s)
      in next_iteration)
   else
     (let
         t = t + 2;
-        ret = t
+        ret = t + n_hashes_acc_imp_after_loop_time 0 s
      in ret)
   )"
   by auto
 termination
-  by (relation "measure (\<lambda>(t,s). n_hashes_n s)") (simp add: n_hashes_state_upd_def)+
+  by (relation "measure (\<lambda>(t,s). n_hashes_acc_n s)")
+    (simp add: n_hashes_acc_imp_subprogram_simps)+
 
-lemmas [simp del] = n_hashes_imp_time.simps
+lemmas n_hashes_acc_imp_subprogram_time_simps =
+  n_hashes_acc_imp_subprogram_simps
+  n_hashes_acc_imp_after_loop_time_def
+  n_hashes_acc_state_upd_time_def
+  n_hashes_acc_imp_compute_loop_condition_time_def
 
-lemma foo:"n_hashes_n s = 0 \<Longrightarrow> n_hashes_imp_time t s = t + 2"
-  by(subst n_hashes_imp_time.simps) simp
+lemmas [simp del] = n_hashes_acc_imp_time.simps
 
-lemma n_hashes_imp_time_acc: "(n_hashes_imp_time (Suc t) s) = Suc (n_hashes_imp_time t s)"
-  by (induction t s rule: n_hashes_imp_time.induct)
-    ((subst (1 2) n_hashes_imp_time.simps); (simp add: n_hashes_state_upd_def))
+lemma n_hashes_acc_imp_time_acc:
+  "(n_hashes_acc_imp_time (Suc t) s) = Suc (n_hashes_acc_imp_time t s)"
+  by (induction t s rule: n_hashes_acc_imp_time.induct)
+    ((subst (1 2) n_hashes_acc_imp_time.simps); (simp add: n_hashes_acc_state_upd_def))
 
-lemma n_hashes_imp_time_acc_2: "(n_hashes_imp_time x s) = x + (n_hashes_imp_time 0 s)"
-  by (induction x arbitrary: s) (simp add: n_hashes_imp_time_acc)+
+lemma n_hashes_acc_imp_time_acc_2:
+  "(n_hashes_acc_imp_time x s) = x + (n_hashes_acc_imp_time 0 s)"
+  by (induction x arbitrary: s) (simp add: n_hashes_acc_imp_time_acc)+
+
+lemma n_hashes_acc_imp_time_acc_2_simp:
+  "(n_hashes_acc_imp_time (n_hashes_state_upd_time 0 s) s') =
+   (n_hashes_state_upd_time 0 s) + (n_hashes_acc_imp_time 0 s')"
+  by (rule n_hashes_acc_imp_time_acc_2)
+
+abbreviation "n_hashes_acc_while_cond \<equiv> ''condition''"
+
+definition "n_hashes_acc_IMP_init_while_cond \<equiv>
+  \<comment> \<open>condition = n_hashes_n s\<close>
+  n_hashes_acc_while_cond ::= (A (V n_hashes_acc_n_str))"
+
+definition "n_hashes_acc_IMP_loop_body \<equiv>
+  \<comment> \<open>cons_h' = hash_as_nat;\<close>
+  ((cons_prefix @ cons_h_str) ::= (A (N 35)));;
+  \<comment> \<open>cons_t' = n_hashes_acc_acc s;\<close>
+  ((cons_prefix @ cons_t_str) ::= (A (V n_hashes_acc_acc_str)));;
+  \<comment> \<open>cons_ret' = 0;\<close>
+  ((cons_prefix @ cons_ret_str) ::= (A (N 0)));;
+  \<comment> \<open>cons_state = \<lparr>cons_h = cons_h', cons_t = cons_t', cons_ret = cons_ret'\<rparr>;\<close>
+  \<comment> \<open>cons_ret_state = cons_imp cons_state;\<close>
+  (invoke_subprogram cons_prefix cons_IMP_Minus);;
+  \<comment> \<open>n_hashes_acc_acc' = cons_ret cons_ret_state;\<close>
+  ((n_hashes_acc_acc_str) ::= (A (V (cons_prefix @ cons_ret_str))));;
+  \<comment> \<open>n_hashes_acc_n' = n_hashes_acc_n s - 1\<close>
+  ((n_hashes_acc_n_str) ::= (Sub (V n_hashes_acc_n_str) (N 1)))"
 
 
-\<comment> \<open>Split IMP- command improve parsing time again.\<close>
-abbreviation "n_hashes_IMP_Minus_1 \<equiv>
-        \<comment> \<open>cons_h' = 35;\<close>
-        ((cons_prefix @ cons_h_str) ::= (A (N 35)));;
-        \<comment> \<open>cons_t' = n_hashes_acc s;\<close>
-        ((cons_prefix @ cons_t_str) ::= (A (V n_hashes_acc_str)));;
-        \<comment> \<open>cons_ret' = 0;\<close>
-        ((cons_prefix @ cons_ret_str) ::= (A (N 0)));;
-        \<comment> \<open>cons_state = \<lparr>cons_h = cons_h', cons_t = cons_t', cons_ret = cons_ret'\<rparr>;\<close>
-        \<comment> \<open>cons_ret_state = cons_imp cons_state;\<close>
-        (invoke_subprogram cons_prefix cons_IMP_Minus)"
+definition "n_hashes_acc_IMP_after_loop \<equiv>
+  \<comment> \<open>ret = s\<close>
+  ((n_hashes_acc_ret_str) ::= (A (V n_hashes_acc_acc_str)))"
 
-definition n_hashes_IMP_Minus where
-  "n_hashes_IMP_Minus \<equiv>
-    (
-    WHILE n_hashes_n_str \<noteq>0 DO
-          n_hashes_IMP_Minus_1;;
-          \<comment> \<open>n_hashes_acc' = cons_ret cons_ret_state;\<close>
-          ((n_hashes_acc_str) ::= (A (V (cons_prefix @ cons_ret_str))));;
-          \<comment> \<open>n_hashes_n' = n_hashes_n s - 1\<close>
-          ((n_hashes_n_str) ::= (Sub (V n_hashes_n_str) (N 1)))
-    )"
+definition n_hashes_acc_IMP_Minus where
+  "n_hashes_acc_IMP_Minus \<equiv>
+  n_hashes_acc_IMP_init_while_cond;;
+  WHILE n_hashes_acc_while_cond \<noteq>0 DO (
+    n_hashes_acc_IMP_loop_body;;
+    n_hashes_acc_IMP_init_while_cond
+  );;
+  n_hashes_acc_IMP_after_loop"
 
-definition "n_hashes_imp_to_HOL_state p s =
-  \<lparr>n_hashes_acc = (s (add_prefix p n_hashes_acc_str)),
-   n_hashes_n = (s (add_prefix p n_hashes_n_str))\<rparr>"
+abbreviation
+  "n_hashes_acc_IMP_vars \<equiv>
+  {n_hashes_acc_acc_str, n_hashes_acc_n_str, n_hashes_acc_ret_str}"
 
-lemma n_hashes_IMP_Minus_correct_function:
-  "(invoke_subprogram p n_hashes_IMP_Minus, s) \<Rightarrow>\<^bsup>t\<^esup> s' \<Longrightarrow>
-     s' (add_prefix p n_hashes_acc_str)
-      = n_hashes_state.n_hashes_acc (n_hashes_imp (n_hashes_imp_to_HOL_state p s))"
-  apply(induction "n_hashes_imp_to_HOL_state p s" arbitrary: s s' t rule: n_hashes_imp.induct)
-  apply(subst n_hashes_imp.simps)
-  apply(simp only: n_hashes_IMP_Minus_def com_add_prefix.simps aexp_add_prefix.simps atomExp_add_prefix.simps invoke_subprogram_append)
-  apply(erule Seq_tE)+
+lemmas n_hashes_acc_IMP_subprogram_simps =
+  n_hashes_acc_IMP_init_while_cond_def
+  n_hashes_acc_IMP_loop_body_def
+  n_hashes_acc_IMP_after_loop_def
+
+definition "n_hashes_acc_imp_to_HOL_state p s =
+  \<lparr>n_hashes_acc_acc = (s (add_prefix p n_hashes_acc_acc_str)),
+   n_hashes_acc_n = (s (add_prefix p n_hashes_acc_n_str)),
+   n_hashes_acc_ret = (s (add_prefix p n_hashes_acc_ret_str))\<rparr>"
+
+lemmas n_hashes_acc_state_translators =
+  cons_imp_to_HOL_state_def
+  n_hashes_acc_imp_to_HOL_state_def
+
+lemmas n_hashes_acc_complete_simps =
+  n_hashes_acc_IMP_subprogram_simps
+  n_hashes_acc_imp_subprogram_simps
+  n_hashes_acc_state_translators
+
+lemma n_hashes_acc_IMP_Minus_correct_function:
+  "(invoke_subprogram p n_hashes_acc_IMP_Minus, s) \<Rightarrow>\<^bsup>t\<^esup> s' \<Longrightarrow>
+     s' (add_prefix p n_hashes_acc_acc_str)
+      = n_hashes_acc_acc (n_hashes_acc_imp (n_hashes_acc_imp_to_HOL_state p s))"
+  apply(induction "n_hashes_acc_imp_to_HOL_state p s" arbitrary: s s' t
+      rule: n_hashes_acc_imp.induct)
+  apply(subst n_hashes_acc_imp.simps)
+  apply(clarsimp simp: n_hashes_acc_IMP_Minus_def)
   apply(erule While_tE)
-  sorry
+   apply(clarsimp simp: n_hashes_acc_IMP_subprogram_simps n_hashes_acc_imp_subprogram_simps
+      n_hashes_acc_state_translators)
+  apply(erule Seq_tE)+
+  apply(dest_com_gen)
+
+    apply(simp only: n_hashes_acc_IMP_init_while_cond_def prefix_simps)
+    apply(force simp: n_hashes_acc_imp_subprogram_simps n_hashes_acc_state_translators)
+
+   apply(clarsimp simp: n_hashes_acc_IMP_subprogram_simps invoke_subprogram_append)
+   apply(erule cons_IMP_Minus_correct[where vars = "n_hashes_acc_IMP_vars"], fastforce)
+   apply (fastforce simp: n_hashes_acc_imp_subprogram_simps n_hashes_acc_state_translators)
+
+  apply(clarsimp simp: n_hashes_acc_IMP_subprogram_simps invoke_subprogram_append)
+  apply(erule cons_IMP_Minus_correct[where vars = "n_hashes_acc_IMP_vars"], fastforce)
+  apply (fastforce simp: n_hashes_acc_imp_subprogram_simps n_hashes_acc_state_translators)
+  done
+
+lemma n_hashes_acc_IMP_Minus_correct_effects:
+  "\<lbrakk>(invoke_subprogram (p @ n_hashes_acc_pref) n_hashes_acc_IMP_Minus, s) \<Rightarrow>\<^bsup>t\<^esup> s';
+    v \<in> vars; \<not> (prefix n_hashes_acc_pref v)\<rbrakk>
+  \<Longrightarrow> s (add_prefix p v) = s' (add_prefix p v)"
+  using com_add_prefix_valid'' com_only_vars prefix_def
+  by blast
+
+lemma n_hashes_acc_IMP_Minus_correct_time_loop_condition:
+  "(invoke_subprogram p n_hashes_acc_IMP_init_while_cond, s) \<Rightarrow>\<^bsup>t\<^esup> s' \<Longrightarrow>
+     t = n_hashes_acc_imp_compute_loop_condition_time 0 (n_hashes_acc_imp_to_HOL_state p s)"
+  by (subst n_hashes_acc_imp_compute_loop_condition_time_def)
+    (auto simp: n_hashes_acc_IMP_init_while_cond_def)
+
+lemmas n_hashes_acc_complete_time_simps =
+  n_hashes_acc_imp_subprogram_time_simps
+  n_hashes_acc_imp_time_acc
+  n_hashes_acc_imp_time_acc_2_simp
+
+lemma n_hashes_acc_IMP_Minus_correct_time:
+  "(invoke_subprogram p n_hashes_acc_IMP_Minus, s) \<Rightarrow>\<^bsup>t\<^esup> s' \<Longrightarrow>
+     t = n_hashes_acc_imp_time 0 (n_hashes_acc_imp_to_HOL_state p s)"
+  apply(induction "n_hashes_acc_imp_to_HOL_state p s" arbitrary: s s' t
+      rule: n_hashes_acc_imp.induct)
+  apply(subst n_hashes_acc_imp_time.simps)
+  apply(clarsimp simp: n_hashes_acc_IMP_Minus_def)
+  apply(erule While_tE_time)
+   apply(clarsimp simp: n_hashes_acc_IMP_subprogram_simps n_hashes_acc_state_translators
+      n_hashes_acc_imp_subprogram_time_simps)
+  apply(clarsimp simp: add.assoc)
+  apply(dest_com_gen_time)
+
+    apply(force simp: n_hashes_acc_IMP_init_while_cond_def n_hashes_acc_imp_subprogram_time_simps
+      n_hashes_acc_state_translators)
+
+   apply(clarsimp simp: n_hashes_acc_IMP_loop_body_def invoke_subprogram_append)
+   apply(erule cons_IMP_Minus_correct[where vars = "n_hashes_acc_IMP_vars"], fastforce)
+   apply (force simp: n_hashes_acc_complete_simps)
+
+  apply(clarsimp simp: n_hashes_acc_IMP_init_while_cond_def n_hashes_acc_IMP_loop_body_def
+      invoke_subprogram_append)
+  apply(erule cons_IMP_Minus_correct[where vars = "n_hashes_acc_IMP_vars"], fastforce)
+  apply(force simp: n_hashes_acc_complete_time_simps n_hashes_acc_state_translators)
+  done
+
+lemma n_hashes_acc_IMP_Minus_correct:
+  "\<lbrakk>(invoke_subprogram (p1 @ p2) n_hashes_acc_IMP_Minus, s) \<Rightarrow>\<^bsup>t\<^esup> s';
+    \<And>v. v \<in> vars \<Longrightarrow> \<not> (set p2 \<subseteq> set v);
+     \<lbrakk>t = (n_hashes_acc_imp_time 0 (n_hashes_acc_imp_to_HOL_state (p1 @ p2) s));
+      s' (add_prefix (p1 @ p2) n_hashes_acc_acc_str) =
+        n_hashes_acc_state.n_hashes_acc_acc (n_hashes_acc_imp (n_hashes_acc_imp_to_HOL_state (p1 @ p2) s));
+      \<And>v. v \<in> vars \<Longrightarrow> s (add_prefix p1 v) = s' (add_prefix p1 v)\<rbrakk>
+     \<Longrightarrow> P\<rbrakk> \<Longrightarrow> P"
+  using n_hashes_acc_IMP_Minus_correct_function
+  by (auto simp: n_hashes_acc_IMP_Minus_correct_time)
+    (meson n_hashes_acc_IMP_Minus_correct_effects set_mono_prefix)
 
 end
